memory_safety/classes.v
@@ -1,0 +1,16 @@
+Require Import common.
+
+Set Implicit Arguments.
+Unset Strict Implicit.
+Unset Printing Implicit Defensive.
+
+Section classes.
+
+Context `{t : machine_types}.
+
+Class memory_syscall_addrs := {
+  malloc_addr : word t;
+  free_addr : word t
+}.
+
+End classes.
