sealing/abstract.v
@@ -6,7 +6,7 @@ Require Import lib.utils.
 Import DoNotation.
 
 Require Import utils common.
-Require Import classes.
+Require Import sealing.classes.
 
 Set Implicit Arguments.
 Unset Strict Implicit.
